figure out how to state lock and use lock invariants in distctr. also converted counter to simply be replicated for now

src/Examples/DistributedCtr/DistCtrImpl.v
@@ -2,73 +2,80 @@ From iris.algebra Require Import auth frac_auth excl.
 From iris.base_logic.lib Require Import invariants.
 From iris.heap_lang Require Import proofmode notation lib.par lib.spin_lock.
 
-Definition alloc : expr :=
+Definition alloc : val :=
+  λ: "()",
   let: "r1" := ref #0 in
   let: "r2" := ref #0 in
-  let: "lk1" := newlock #() in
-  let: "lk2" := newlock  #() in
-  Pair (Pair "r1" "r2") (Pair "lk1" "lk2").
+  let: "lk" := newlock #() in
+  Pair (Pair "r1" "r2") "lk".
 
 (* precondition: r1 r2 are an alloced pair *)
-Definition inc (rpair : expr) (lkpair: expr) : expr :=
-  let: "r1" := Fst rpair in
-  let: "r2" := Snd rpair in
-  let: "lk1" := Fst lkpair in
-  let: "lk2" := Snd lkpair in
-  (
-    (acquire "lk1";; "r1" <- !"r1" + #1;; release "lk1")
+Definition inc : val :=
+  λ: "rpair" "lk",
+  let: "r1" := Fst "rpair" in
+  let: "r2" := Snd "rpair" in
+  acquire "lk";;
+  (("r1" <- !"r1" + #1)
   |||
-    (acquire "lk2";; "r2" <- !"r2" + #2;; release "lk2")
-  ).
+  ("r2" <- !"r2" + #1))
+  release "lk".
 
-Definition sum (rpair : expr) (lkpair: expr) : expr :=
-  let: "r1" := Fst rpair in
-  let: "r2" := Snd rpair in
-  let: "lk1" := Fst lkpair in let: "lk2" := Snd lkpair in acquire "lk1";; acquire "lk2";;
+Definition sum : val :=
+  λ: "rpair" "lk",
+  let: "r1" := Fst "rpair" in
+  let: "r2" := Snd "rpair" in
+  acquire "lk";;
   "r" <-!"r1" + !"r2";;
-  release "lk2";; release "lk1";;
+  release "lk";;
   "r".
 
 Section proof.
   (** Come up with a suitable invariant and prove the spec **)
-  Context `{!heapG Σ, !spawnG Σ, !inG Σ (authR (optionUR (exclR ZO)))}.
+  Context `{!heapG Σ, !spawnG Σ, !lockG Σ, !inG Σ (authR (optionUR (exclR ZO)))}.
+  Definition LockN : namespace := nroot .@ "LockN".
 
-  Definition parallel_add_inv (rpair : loc * loc) : iProp Σ := (*(γ1 γ2 : gname) : iProp Σ :=*)
+  Definition parallel_inc_inv (rpair : loc * loc) : iProp Σ := (*(γ1 γ2 : gname) : iProp Σ :=*)
     (∃ n1 n2:Z, (⌜#n1 = #n2⌝
                   ∗ (fst rpair) ↦ #(n1))
                   ∗ ((snd rpair) ↦ #(n2))%I).
                   (*∗ own γ1 (● (Excl' n1)) ∗ own γ2 (● (Excl' n2)))%I.*)
 
   (* Notes: loc = kind of like a Coq literal number, LitV (LitLoc loc) is an actual value in the language *)
-  Definition pair_eq (n: Z) (rpair : loc * loc) : iProp Σ := (fst rpair) ↦ #n ∗ (snd rpair) ↦ #n.
 
-  Print val . 
-  Locate "#".
-  Print base_lit. 
-
-  Implicit Types (l: loc).
   Lemma alloc_spec : 
     {{{ True%I }}}
-      alloc
-    {{{ l1 l2 lk1 lk2, RET PairV (PairV #l1 #l2) (PairV #lk1 #lk2); pair_eq 0 (l1, l2) }}}.
+      alloc #()
+      {{{ r1 r2 lk, RET PairV (PairV #r1 #r2) #lk; parallel_inc_inv (r1, r2) ∗ ∃ γ, is_lock LockN γ #lk (parallel_inc_inv (r1, r2))}}}.
+  (* DO I NEED FORALL OR EXISTS GAMMA *)
   Proof.
     iIntros (Φ) "_ HPost".
     unfold alloc.
     wp_alloc r1 as "Hr1".
     wp_alloc r2 as "Hr2"; wp_let; wp_lam.
-    wp_alloc lk1 as "Hlk1"; wp_let; wp_lam.
-    wp_alloc lk2 as "Hlk2"; wp_let.
+    wp_alloc lk as "Hlk"; wp_let.
     wp_pures.
     iApply "HPost".
-    unfold pair_eq; simpl in *; iFrame; auto.
+
   Qed.
 
-  Lemma inc_spec : ∀ n rpair lpair,
-    {{{ pair_eq n rpair }}}
-      inc (#(fst rpair), #(snd rpair)) lpair
-    {{{ z, RET #z; pair_eq (n+1) rpair }}}.
+  Print wp_par.
+  Print is_lock.
+  Lemma inc_spec : ∀ n r1 r2 lk1 lk2 R1 R2,
+    {{{ is_lock lk1 R1 ∗ is_lock lk2 R2 ∗ pair_eq n (r1, r2)}}}
+      inc (#r1, #r2) (#lk1, #lk2) 
+    {{{ z, RET #z; pair_eq (n+1) (r1, r2)}}}.
   Proof.
-    (* exercise *)
+    iIntros (n r1 r2 lk1 lk2 ϕ) "HPair Hϕ".
+    unfold inc.
+    unfold pair_eq in *.
+    wp_pures.
+    destruct r1; destruct r2.
+    wp_apply (wp_par (λ _, True%I) (λ _, True%I)).
+    Print acquire_spec.
+    - wp_apply (acquire_spec). iDestruct 1 as (n) "[Hr %]"
+    unfold acquire in *.
+    wp_pures.
+    wp_alloc r1 as "Hr1".
   Admitted.
 
   Lemma sum_spec : ∀ n rpair lpair,
@@ -76,6 +83,5 @@ Section proof.
       sum (#(fst rpair), #(snd rpair)) lpair
     {{{ z, RET #z; ⌜ z = (n + n)%Z ⌝ }}}.
   Proof.
-    (* exercise *)
   Admitted.
 End proof.
