src/Examples/solutions/ex_04_parallel_add.v
@@ -1,0 +1,195 @@
+(**
+In this exercise we use the spin-lock from the previous exercise to implement
+the running example during the lecture of the tutorial: proving that when two
+threads increase a reference that's initially zero by two, the result is four.
+*)
+From iris.algebra Require Import auth frac_auth excl.
+From iris.base_logic.lib Require Import invariants.
+From iris.heap_lang Require Import lib.par proofmode notation lib.spin_lock.
+
+(** The program as a heap-lang expression. We use the heap-lang [par] module for
+parallel composition. *)
+Definition parallel_add : expr :=
+  let: "r" := ref #0 in
+  let: "l" := newlock #() in
+  (
+    (acquire "l";; "r" <- !"r" + #2;; release "l")
+  |||
+    (acquire "l";; "r" <- !"r" + #2;; release "l")
+  );;
+  acquire "l";;
+  !"r".
+
+Section proof1.
+  Context `{!heapG Σ, !spawnG Σ, !lockG Σ}.
+
+  Definition parallel_add_inv_1 (r : loc) : iProp Σ :=
+    (∃ n : Z, r ↦ #n ∗ ⌜ Zeven n ⌝)%I.
+
+  (** *Exercise*: finish the missing cases of this proof. *)
+  Print namespace.
+  Definition LockN : namespace := nroot .@ "LockN".
+  Lemma parallel_add_spec_1 :
+    {{{ True }}} parallel_add {{{ n, RET #n; ⌜Zeven n⌝ }}}.
+  Proof.
+    iIntros (Φ) "_ Post".
+    unfold parallel_add. wp_alloc r as "Hr". wp_let.
+    Check newlock_spec.
+    iDestruct (newlock_spec LockN (parallel_add_inv_1 r) with "[Hr]") as "H".
+    unfold parallel_add_inv_1.
+    iExists 0; iFrame; auto.
+
+    wp_apply "H".
+    iIntros (l γ) "#Hl". wp_let.
+    wp_apply (wp_par (λ _, True%I) (λ _, True%I)).
+    - wp_apply (acquire_spec with "Hl").
+      iIntros "(Hlocked & H)".
+      iDestruct "H" as (n) "[Hr %]".
+      wp_seq. wp_load. wp_op. wp_store.
+      wp_apply (release_spec with "[Hr $Hl $Hlocked]"); [|done].
+      iExists _. iFrame "Hr". iPureIntro. by apply Zeven_plus_Zeven.
+    - wp_apply (acquire_spec with "Hl").
+      iIntros "(Hlocked & H)".
+      iDestruct "H" as (n) "[Hr %]".
+      wp_seq. wp_load. wp_op. wp_store.
+      wp_apply (release_spec with "[Hr $Hl $Hlocked]"); [|done].
+      iExists _. iFrame "Hr". iPureIntro. by apply Zeven_plus_Zeven.
+    - iIntros (v1 v2) "_ !>". wp_seq.
+      wp_apply (acquire_spec with "Hl").
+      iIntros "(Hlocked & H)". iDestruct "H" as (n) "[Hr %]".
+      wp_seq. wp_load. by iApply "Post".
+  Qed.
+End proof1.
+
+(** 2nd proof : we prove that the program returns 4 exactly.
+We need a piece of ghost state: integer ghost variables.
+
+Whereas we previously abstracted over an arbitrary "ghost state" [Σ] in the
+proofs, we now need to make sure that we can use integer ghost variables. For
+this, we add the type class constraint:
+
+  inG Σ (authR (optionUR (exclR ZO)))
+
+*)
+
+Section proof2.
+  Context `{!heapG Σ, !spawnG Σ, !lockG Σ, !inG Σ (authR (optionUR (exclR ZO)))}.
+
+  Definition parallel_add_inv_2 (r : loc) (γ1 γ2 : gname) : iProp Σ :=
+    (∃ n1 n2 : Z, r ↦ #(n1 + n2)
+            ∗ own γ1 (● (Excl' n1)) ∗ own γ2 (● (Excl' n2)))%I.
+
+  (** Some helping lemmas for ghost state that we need in the proof. In actual
+  proofs we tend to inline simple lemmas like these, but they are here to
+  make things easier to understand. *)
+  Lemma ghost_var_alloc n :
+    (|==> ∃ γ, own γ (● (Excl' n)) ∗ own γ (◯ (Excl' n)))%I.
+  Proof.
+    iMod (own_alloc (● (Excl' n) ⋅ ◯ (Excl' n))) as (γ) "[??]".
+    - by apply auth_both_valid.
+    - by eauto with iFrame.
+  Qed.
+
+  Lemma ghost_var_agree γ n m :
+    own γ (● (Excl' n)) -∗ own γ (◯ (Excl' m)) -∗ ⌜ n = m ⌝.
+  Proof.
+    iIntros "Hγ● Hγ◯".
+    Check own_valid_2.
+    by iDestruct (own_valid_2 with "Hγ● Hγ◯")
+      as %[<-%Excl_included%leibniz_equiv _]%auth_both_valid.
+    (* XXX What is this last line doing??? *)
+  Qed.
+
+  Lemma ghost_var_update γ n' n m :
+    own γ (● (Excl' n)) -∗ own γ (◯ (Excl' m)) ==∗
+      own γ (● (Excl' n')) ∗ own γ (◯ (Excl' n')).
+  Proof.
+    iIntros "Hγ● Hγ◯".
+    iMod (own_update_2 _ _ _ (● Excl' n' ⋅ ◯ Excl' n') with "Hγ● Hγ◯") as "[$$]".
+    { apply auth_update. apply option_local_update. apply exclusive_local_update. done. }
+    (* ??? *)
+    done.
+  Qed.
+
+  (** *Exercise*: finish the missing cases of the proof. *)
+  Lemma parallel_add_spec_2 :
+    {{{ True }}} parallel_add {{{ RET #4; True }}}.
+  Proof.
+    iIntros (Φ) "_ Post".
+    unfold parallel_add. wp_alloc r as "Hr". wp_let.
+    iMod (ghost_var_alloc 0) as (γ1) "[Hγ1● Hγ1◯]".
+    iMod (ghost_var_alloc 0) as (γ2) "[Hγ2● Hγ2◯]".
+    iDestruct (newlock_spec LockN (parallel_add_inv_2 r γ1 γ2) with "[Hr Hγ1● Hγ2●]") as "H".
+    { (* exercise *) iExists 0, 0. iFrame. }
+    wp_apply "H".
+    iIntros (l γ) "#Hl". wp_let.
+    wp_apply (wp_par (λ _, own γ1 (◯ Excl' 2)) (λ _, own γ2 (◯ Excl' 2))
+                with "[Hγ1◯] [Hγ2◯]").
+    - wp_apply (acquire_spec with "Hl"). iIntros "(Hlked & H)". iDestruct "H" as (n1 n2) "(Hr & Hγ1● & Hγ2●)".
+      wp_seq. wp_load. wp_op. wp_store.
+      iDestruct (ghost_var_agree with "Hγ1● Hγ1◯") as %->.
+      iMod (ghost_var_update γ1 2 with "Hγ1● Hγ1◯") as "[Hγ1● Hγ1◯]".
+      wp_apply (release_spec with "[- $Hl Hγ1◯]"); [|by auto].
+      (* WHAT DOES - MEAN *)
+      iFrame.
+      iExists _, _. iFrame "Hγ1● Hγ2●". rewrite (_ : 2 + n2 = 0 + n2 + 2); [done | ring]. (* this does arithmetic *)
+    - wp_apply (acquire_spec with "Hl").
+      iIntros "(HLked & H)". iDestruct "H" as (n1 n2) "(Hr & Hγ1● & Hγ2●)".
+      wp_seq. wp_load. wp_op. wp_store.
+      iDestruct (ghost_var_agree with "Hγ2● Hγ2◯") as %->.
+      iMod (ghost_var_update γ2 2 with "Hγ2● Hγ2◯") as "[Hγ2● Hγ2◯]".
+      wp_apply (release_spec with "[- $Hl Hγ2◯]"); [|by auto].
+      iFrame. iExists _, _. iFrame "Hγ1● Hγ2●". by rewrite -Z.add_assoc.
+    - iIntros (??) "[Hγ1◯ Hγ2◯] !>". wp_seq.
+      wp_apply (acquire_spec with "Hl"). iIntros "(Hlk & H)". iDestruct "H" as (n1 n2) "(Hr & Hγ1● & Hγ2●)".
+      wp_seq. wp_load.
+      iDestruct (ghost_var_agree with "Hγ1● Hγ1◯") as %->.
+      iDestruct (ghost_var_agree with "Hγ2● Hγ2◯") as %->.
+      by iApply "Post".
+  Qed.
+End proof2.
+
+(** 3rd proof : we prove that the program returns 4 exactly, but using a
+fractional authoritative ghost state.  We need another piece of ghost state. *)
+Section proof3.
+  Context `{!heapG Σ, !spawnG Σ, !inG Σ (frac_authR natR)}.
+
+  Definition parallel_add_inv_3 (r : loc) (γ : gname) : iProp Σ :=
+    (∃ n : nat, r ↦ #n ∗ own γ (●F n))%I.
+
+  (** *Exercise*: finish the missing cases of the proof. *)
+  Lemma parallel_add_spec_3 :
+    {{{ True }}} parallel_add {{{ RET #4; True }}}.
+  Proof.
+    iIntros (Φ) "_ Post".
+    unfold parallel_add. wp_alloc r as "Hr". wp_let.
+    iMod (own_alloc (●F 0%nat ⋅ ◯F 0%nat)) as (γ) "[Hγ● [Hγ1◯ Hγ2◯]]".
+    { by apply auth_both_valid. }
+    wp_apply (newlock_spec (parallel_add_inv_3 r γ) with "[Hr Hγ●]").
+    { (* exercise *) iExists 0%nat. iFrame. }
+    iIntros (l) "#Hl". wp_let.
+    wp_apply (wp_par (λ _, own γ (◯F{1/2} 2%nat)) (λ _, own γ (◯F{1/2} 2%nat))
+                with "[Hγ1◯] [Hγ2◯]").
+    - wp_apply (acquire_spec with "Hl"). iDestruct 1 as (n) "[Hr Hγ●]".
+      wp_seq. wp_load. wp_op. wp_store.
+      iMod (own_update_2 _ _ _ (●F (n+2) ⋅ ◯F{1/2}2)%nat with "Hγ● Hγ1◯") as "[Hγ● Hγ1◯]".
+      { rewrite (comm plus).
+        by apply frac_auth_update, (op_local_update_discrete n 0 2)%nat. }
+      wp_apply (release_spec with "[$Hl Hr Hγ●]"); [|by auto].
+      iExists _. iFrame. by rewrite Nat2Z.inj_add.
+    - (* exercise *)
+      wp_apply (acquire_spec with "Hl"). iDestruct 1 as (n) "[Hr Hγ●]".
+      wp_seq. wp_load. wp_op. wp_store.
+      iMod (own_update_2 _ _ _ (●F (n+2) ⋅ ◯F{1/2}2)%nat with "Hγ● Hγ2◯") as "[Hγ● Hγ2◯]".
+      { rewrite (comm plus).
+        by apply frac_auth_update, (op_local_update_discrete n 0 2)%nat. }
+      wp_apply (release_spec with "[- $Hl Hγ2◯]"); [|by auto].
+      iExists _. iFrame. by rewrite Nat2Z.inj_add.
+    - (* exercise *)
+      iIntros (??) "[Hγ1◯ Hγ2◯] !>". wp_seq.
+      wp_apply (acquire_spec with "Hl"). iDestruct 1 as (n) "(Hr & Hγ●)".
+      wp_seq. wp_load. iCombine "Hγ1◯ Hγ2◯" as "Hγ◯".
+      iDestruct (own_valid_2 with "Hγ● Hγ◯") as %->%frac_auth_agreeL.
+      by iApply "Post".
+  Qed.
+End proof3.
