src/Examples/solutions/ex_05_parallel_add_mul.v
@@ -1,0 +1,107 @@
+(**
+In this exercise we consider a variant of the previous exercise. We have a
+reference which is initially 0 and two threads running in parallel. One thread
+increases the value of the reference by 2, whereas the other multiples the
+value of the reference by two. An interesting aspect of this exercise is that
+the outcome of this program is non-deterministic. Depending on which thread runs
+first, the outcome is either 2 or 4.
+
+Contrary to the earlier exercises, this exercise is nearly entirely open.
+*)
+From iris.algebra Require Import auth frac_auth excl.
+From iris.base_logic.lib Require Import invariants.
+From iris.heap_lang Require Import proofmode notation lib.par.
+Require Import solutions.ex_03_spinlock.
+
+Definition parallel_add_mul : expr :=
+  let: "r" := ref #0 in
+  let: "l" := newlock #() in
+  (
+    (acquire "l";; "r" <- !"r" + #2;; release "l")
+  |||
+    (acquire "l";; "r" <- !"r" * #2;; release "l")
+  );;
+  acquire "l";;
+  !"r".
+
+(** In this proof we will make use of Boolean ghost variables. *)
+Section proof.
+  Context `{!heapG Σ, !spawnG Σ, !inG Σ (authR (optionUR (exclR boolO)))}.
+
+  (** The same helping lemmas for ghost variables that we have already seen in
+  the previous exercise. *)
+  Lemma ghost_var_alloc b :
+    (|==> ∃ γ, own γ (● (Excl' b)) ∗ own γ (◯ (Excl' b)))%I.
+  Proof.
+    iMod (own_alloc (● (Excl' b) ⋅ ◯ (Excl' b))) as (γ) "[??]".
+    - by apply auth_both_valid.
+    - by eauto with iFrame.
+  Qed.
+
+  Lemma ghost_var_agree γ b c :
+    own γ (● (Excl' b)) -∗ own γ (◯ (Excl' c)) -∗ ⌜ b = c ⌝.
+  Proof.
+    iIntros "Hγ● Hγ◯".
+    by iDestruct (own_valid_2 with "Hγ● Hγ◯")
+      as %[<-%Excl_included%leibniz_equiv _]%auth_both_valid.
+  Qed.
+
+  Lemma ghost_var_update γ b' b c :
+    own γ (● (Excl' b)) -∗ own γ (◯ (Excl' c)) ==∗
+      own γ (● (Excl' b')) ∗ own γ (◯ (Excl' b')).
+  Proof.
+    iIntros "Hγ● Hγ◯".
+    iMod (own_update_2 _ _ _ (● Excl' b' ⋅ ◯ Excl' b') with "Hγ● Hγ◯") as "[$$]".
+    { by apply auth_update, option_local_update, exclusive_local_update. }
+    done.
+  Qed.
+
+  (** *Difficult exercise*: come up with a suitable invariant and prove the spec
+  of [parallel_add_mul]. In this proof, you should use Boolean ghost variables,
+  and the rules for those as given above. You are allowed to use any number of
+  Boolean ghost variables. *)
+  Definition parallel_add_mul_inv (r : loc) (γ1 γ2 : gname) : iProp Σ :=
+    (∃ (b1 b2 : bool) (z : Z),
+        own γ1 (● Excl' b1) ∗ own γ2 (● Excl' b2) ∗ r ↦ #z ∗
+       ⌜match b1, b2 with
+        | true,  true  => z = 2 ∨ z = 4
+        | true,  false => z = 2
+        | false, _     => z = 0
+        end⌝)%I.
+
+  Lemma parallel_add_mul_spec :
+    {{{ True }}} parallel_add_mul {{{ z, RET #z; ⌜ z = 2 ∨ z = 4 ⌝ }}}.
+  Proof.
+    iIntros (Φ) "_ Post".
+    unfold parallel_add_mul. wp_alloc r as "Hr". wp_let.
+    iMod (ghost_var_alloc false) as (γ1) "[Hγ1● Hγ1◯]".
+    iMod (ghost_var_alloc false) as (γ2) "[Hγ2● Hγ2◯]".
+    wp_apply (newlock_spec (parallel_add_mul_inv r γ1 γ2) with "[Hr Hγ1● Hγ2●]").
+    { iExists false, false, 0. iFrame. done. }
+    iIntros (l) "#Hl". wp_let.
+    wp_apply (wp_par (λ _, own γ1 (◯ Excl' true)) (λ _, own γ2 (◯ Excl' true))
+                with "[Hγ1◯] [Hγ2◯]").
+    - wp_apply (acquire_spec with "Hl").
+      iDestruct 1 as (b1 b2 z) "(Hγ1● & Hγ2● & Hr & %)".
+      wp_seq. wp_load. wp_op. wp_store.
+      iDestruct (ghost_var_agree with "Hγ1● Hγ1◯") as %->. subst z.
+      iMod (ghost_var_update γ1 true with "Hγ1● Hγ1◯") as "[Hγ1● Hγ1◯]".
+      wp_apply (release_spec with "[- $Hl Hγ1◯]"); [|by auto].
+      iExists _, _, _. iFrame "Hγ1● Hγ2● Hr". destruct b2; auto.
+    - wp_apply (acquire_spec with "Hl").
+      iDestruct 1 as (b1 b2 z) "(Hγ1● & Hγ2● & Hr & %)".
+      wp_seq. wp_load. wp_op. wp_store.
+      iDestruct (ghost_var_agree with "Hγ2● Hγ2◯") as %->.
+      iMod (ghost_var_update γ2 true with "Hγ2● Hγ2◯") as "[Hγ2● Hγ2◯]".
+      wp_apply (release_spec with "[$Hl Hγ1● Hr Hγ2●]"); [|by auto].
+      iExists _, _, _. iFrame "Hγ1● Hγ2● Hr". destruct b1; subst z; auto.
+    - iIntros (??) "[Hγ1◯ Hγ2◯] !>". wp_seq.
+      wp_apply (acquire_spec with "Hl").
+      iDestruct 1 as (b1 b2 z) "(Hγ1● & Hγ2● & Hr & %)".
+      wp_seq. wp_load.
+      iApply "Post".
+      iDestruct (ghost_var_agree with "Hγ1● Hγ1◯") as %->.
+      iDestruct (ghost_var_agree with "Hγ2● Hγ2◯") as %->.
+      auto.
+  Qed.
+End proof.
