src/ShouldBuild.v
@@ -7,6 +7,7 @@ From Perennial Require Import Examples.AtomicPair.RefinementLog.
 (* From Perennial Require Import Examples.Logging2.RefinementLog2. *)
 From Perennial Require Import Examples.ReplicatedDisk.ReplicatedDiskRefinement.
 From Perennial Require Import Examples.DistributedCtr.DistCtrImpl.
+From Perennial Require Import Examples.solutions.ex_04_parallel_add.
 
 (* mailboat proof *)
 From Perennial Require Import Examples.MailServer.MailRefinement.
